examples/litmus/tools/bir_promisingExecSimScript.sml
@@ -1,0 +1,358 @@
+open HolKernel Parse boolLib bossLib;
+open bir_promisingTheory bir_promisingExecScript bir_programTheory;
+open listTheory arithmeticTheory;
+open bir_expTheory;
+open numeralTheory arithmeticTheory;
+open pred_setTheory;
+open BasicProvers listRangeTheory;
+open rich_listTheory;
+open prim_recTheory
+
+val _ = new_theory "bir_promisingExecSim";
+
+Theorem MAXL_LE:
+  ∀xs y.
+  MAXL xs ≤ y ⇔ EVERY (\x. x ≤ y) xs
+Proof
+  cheat
+QED
+
+Triviality EL_SNOC2:
+  ∀x l.
+    EL (LENGTH l) (SNOC x l) = x
+Proof
+  Induct_on ‘l’ >>
+  (asm_rewrite_tac [LENGTH, SNOC, EL, HD, TL])
+QED
+
+Triviality zip_memory_ts:
+  ∀m t M.
+  MEM (m, t) (ZIP (M, [1 .. LENGTH M])) = (t ≠ 0 ∧ oEL (PRE t)  M = SOME m)
+Proof
+  Induct_on ‘M’ using SNOC_INDUCT >|
+  [
+    fs [listRangeINC_def, oEL_def]
+    ,
+    fs [GENLIST, listRangeINC_def, ZIP_SNOC, oEL_THM] >>
+    rpt gen_tac >>
+    eq_tac >|
+    [
+      rpt strip_tac >>
+      (fs [LESS_THM, EL_SNOC2, GSYM ADD1, EL_SNOC])
+      ,
+      rpt strip_tac >>
+      gvs [oEL_THM, LESS_THM, EL_SNOC, EL_SNOC2]
+    ]
+  ]
+QED
+
+Triviality EVERY_oEL:
+  ∀P l.
+  EVERY P l ⇔ ∀x n. oEL n l = SOME x ⇒ P x 
+Proof
+  fs [EVERY_EL, oEL_THM]
+QED
+
+Theorem mem_every_thm:
+  ∀P M.
+  mem_every P M = ∀m t. t ≠ 0 ∧ oEL (PRE t) M = SOME m ⇒ P (m, t)
+Proof
+  rpt gen_tac >>
+  eq_tac >|
+  [
+    Induct_on ‘M’ using SNOC_INDUCT >|
+    [
+      fs [mem_every_def, oEL_THM, listRangeINC_def]
+      ,
+      fs [mem_every_def, oEL_THM, listRangeINC_def, ZIP_SNOC, GENLIST, EVERY_SNOC] >>
+      rpt strip_tac >>
+      fs [LESS_THM] >|
+      [
+        Cases_on ‘t’ >>
+        (fs [GSYM ADD1, EL_SNOC, EL_SNOC2])
+        ,
+        fs [EL_SNOC]
+      ]
+    ]
+    ,
+    rpt strip_tac >>
+    fs [mem_every_def, EVERY_MEM] >>
+    gen_tac >>
+    Cases_on ‘e’ >> rename1 ‘P (x, t)’ >>
+    Cases_on ‘t’ >> (fs[zip_memory_ts])
+  ]
+QED
+
+Theorem MEM_LIST_BIND:
+  ∀e f ll.
+  MEM e (LIST_BIND ll f) ⇔ EXISTS (\l. MEM e (f l)) ll 
+Proof
+  Induct_on ‘ll’ >> (fs [])
+QED
+
+Theorem mem_filter_thm:
+∀P M m t.
+  MEM (m, t) (mem_filter P M) = (P (m, t) ∧ t ≠ 0 ∧ oEL (PRE t) M = SOME m)
+Proof
+  fs [mem_filter_def, MEM_FILTER, zip_memory_ts]
+QED                           
+
+                              open optionTheory;
+Theorem mem_get_SOME_thm:
+  ∀M l t m.
+    mem_get M l t = SOME m ⇔ ((t = 0 ∧ m = mem_default l) ∨ (t ≠ 0 ∧ oEL (PRE t) M = SOME m ∧ m.loc = l))
+Proof
+  rpt gen_tac >>
+  Cases_on ‘t’ >|
+  [
+    fs [mem_get_def, EQ_SYM_EQ]
+    ,
+    fs [mem_get_def, CaseEq"option"]
+  ]
+QED
+
+Theorem mem_get_NONE_thm:
+  ∀M l t.
+    mem_get M l t = NONE ⇔ (t > LENGTH M ∨ (t ≠ 0 ∧ t ≤ LENGTH M ∧ (EL (PRE t) M).loc ≠ l))
+Proof
+  rpt gen_tac >>
+  Cases_on ‘t’ >|
+  [
+    fs [mem_get_def]
+    ,
+    eq_tac >|
+    [
+      rpt strip_tac >>
+      gvs [mem_get_def, oEL_THM, CaseEq"option"]
+      ,
+      rpt strip_tac >|
+      [
+        fs [mem_get_def, CaseEq"option", oEL_THM]
+        ,
+        fs [mem_get_def, CaseEq"option", oEL_THM]
+      ]
+    ]
+  ]
+QED
+
+Theorem MEM_readable_thm:
+  ∀m t M v_max l.
+    MEM (m, t) (mem_readable M l v_max)
+    = (mem_get M l t = SOME m ∧
+       ∀t'. t < t' ∧ t' ≤ v_max ⇒ mem_get M l t' = NONE)
+Proof
+  rpt strip_tac >>
+  eq_tac >|
+  [ (* soundness *)
+    rewrite_tac [mem_readable_def, MEM_FILTER] >>
+    rpt strip_tac >|
+    [
+      Cases_on ‘t’ >>
+      (fs [mem_get_SOME_thm, mem_filter_thm])
+      ,
+      fs [mem_get_NONE_thm, mem_every_thm, oEL_THM] >>
+      (Cases_on ‘t' > LENGTH M’ >|
+      [
+        fs []
+        ,
+        fs [NOT_GREATER]
+      ])
+    ]
+    , (* completeness *)
+    rewrite_tac [mem_readable_def, MEM_FILTER, MEM] >>
+    rpt strip_tac >|
+    [
+      fs [mem_every_thm] >>
+      rpt strip_tac >>
+      first_x_assum drule >>
+      fs [oEL_THM, mem_get_NONE_thm]
+      ,
+      fs [mem_every_thm, mem_filter_thm] >>
+      Cases_on ‘t’ >>
+      (fs [mem_default_def, mem_get_def, CaseEq"option"])
+    ]
+  ]
+QED
+
+Theorem MEM_MAP_PARTIAL2:
+∀x f l.
+  MEM x (MAP_PARTIAL f l)
+  ⇔
+  ∃x'. SOME x = f x' ∧ MEM x' l
+Proof
+  fs [MEM_MAP_PARTIAL, MEM_MAP]
+QED
+
+Theorem mem_read_get:
+  ∀M l t.
+    mem_read M l t =
+    case mem_get M l t of
+    | SOME msg => SOME msg.val
+    | NONE => NONE
+Proof
+  Cases_on ‘t’ >|
+  [
+    fs [mem_read_def, mem_get_def, mem_default_def, mem_default_value_def]
+    ,
+    fs [mem_read_def, mem_get_def]
+    rpt gen_tac >> CASE_TAC >|
+    [
+      fs [mem_read_aux_def, mem_read_def, mem_get_def]
+      ,
+      fs [mem_read_def, mem_read_aux_def] >>
+      CASE_TAC
+    ]
+  ]
+QED
+                   
+
+
+Theorem eval_clstep_read_soundness:
+  ∀p cid M s s' var e acq rel xcl cast.
+  bir_get_stmt p s.bst_pc = BirStmt_Read var e cast acq rel xcl ⇒
+  MEM s' (eval_clstep_read s M var e acq rel xcl) ⇒ clstep p cid s M [] s'
+Proof
+  rpt strip_tac >>
+  fs [clstep_cases, eval_clstep_read_def, bir_state_t_component_equality, bir_eval_exp_view_def] >>
+  Cases_on ‘bir_eval_exp e s.bst_environ’ >|
+  [
+    (* SOME l = NONE *)
+    fs [CaseEq"option"]
+    ,
+    (* SOME l = SOME x *)
+    fs [CaseEq"option"] >>
+    (* MEM s' (MAP_PARTIAL (λ(msg,t). state option) (mem_readable M x (MAX ...)) *)
+    fs [MEM_MAP_PARTIAL2] >>
+    rename1 ‘MEM x' (mem_readable _ _ _)’ >>
+    Cases_on ‘x'’ >>
+    fs [MEM_readable_thm] >>
+    rename1 ‘mem_get M l t = SOME msg’ >>
+    Q.EXISTS_TAC ‘msg.val’ >> Q.EXISTS_TAC ‘t’ >>
+    fs [mem_read_def]
+
+
+QED                                   
+
+
+Theorem eval_clstep_expr_soundness:
+  ∀p cid M s s' var e.
+  bir_get_stmt p s.bst_pc = BirStmt_Expr var e ⇒
+  MEM s' (eval_clstep_exp s var e) ⇒ clstep p cid s M [] s'
+Proof
+  rpt strip_tac >>
+  fs [clstep_cases, eval_clstep_exp_def] >>
+  rpt (FULL_CASE_TAC >> fs [bir_get_stmt_expr])
+QED                                              
+
+Theorem eval_clstep_fence_soundness:
+  ∀p cid M s s' K1 K2.
+  bir_get_stmt p s.bst_pc = BirStmt_Fence K1 K2 ⇒
+  MEM s' (eval_clstep_fence s K1 K2) ⇒ clstep p cid s M [] s'
+Proof
+  rpt strip_tac >>
+  fs [clstep_cases, eval_clstep_fence_def, bir_state_t_component_equality] >>
+  rpt FULL_CASE_TAC >>
+  (fs [] >> METIS_TAC [MAX_COMM])
+QED
+
+Theorem eval_clstep_branch_soundness:
+  ∀p cid M s s' cond_e lbl1 lbl2.
+  bir_get_stmt p s.bst_pc = BirStmt_Branch cond_e lbl1 lbl2 ⇒
+  MEM s' (eval_clstep_branch p s cond_e lbl1 lbl2) ⇒ clstep p cid s M [] s'
+Proof
+  rpt strip_tac >>
+  fs [clstep_cases, eval_clstep_branch_def, bir_state_t_component_equality] >>
+  Cases_on ‘bir_exec_stmt p (BStmtE (BStmt_CJmp cond_e lbl1 lbl2)) s’ >>
+  Cases_on ‘bir_eval_exp_view cond_e s.bst_environ s.bst_viewenv’ >>
+  fs [] >>
+  FULL_CASE_TAC >>
+  (fs [])
+QED
+
+Theorem eval_clstep_bir_step_soundness:
+  ∀p cid M s s' stmt.
+  bir_get_stmt p s.bst_pc = BirStmt_Generic stmt ⇒
+  MEM s' (eval_clstep_bir_step p s stmt) ⇒ clstep p cid s M [] s'
+Proof
+  rpt strip_tac >>
+  fs [clstep_cases, eval_clstep_bir_step_def, bir_state_t_component_equality] >>
+  Cases_on ‘bir_exec_stmt p stmt s’ >>
+  fs []
+QED
+
+Theorem eval_clstep_soundness:
+  ∀p cid M l s s'.
+  MEM s' (eval_clstep cid p s M) ⇒ ∃l. clstep p cid s M l s'
+Proof
+  rpt strip_tac >>
+  fs [eval_clstep_def] >>
+  Cases_on ‘bir_get_stmt p s.bst_pc’ >> (fs []) >|
+  [
+    (* read *)
+    Q.EXISTS_TAC ‘[]’ >>
+    fs [eval_clstep_read_soundness]
+    ,
+    (* fulfil *)
+    cheat
+    ,
+    (* xclfail *)
+    cheat
+    ,
+    (* amofulfil *)
+    cheat
+    ,
+    (* expr *)
+    Q.EXISTS_TAC ‘[]’ >>
+    fs [eval_clstep_expr_soundness]
+    ,
+    (* fence *)
+    Q.EXISTS_TAC ‘[]’ >>
+    fs [eval_clstep_fence_soundness]
+    ,
+    (* branch *)
+    Q.EXISTS_TAC ‘[]’ >>
+    fs [eval_clstep_branch_soundness]
+    ,
+    (* bir_step *)
+    Q.EXISTS_TAC ‘[]’ >>
+    fs [eval_clstep_bir_step_soundness]
+  ]
+QED
+
+Theorem eval_clstep_completeness:
+  ∀p cid s M l s'.
+   clstep p cid s M l s' ⇒ MEM s' (eval_clstep cid p s M)
+Proof
+  rewrite [eval_clstep_def, clstep_cases, ABS_SIMP] >>
+  rpt strip_tac >|
+  [
+    fs [mem_default_def]
+    ,
+    fs []
+    ,
+    fs [mem_filter_thm]
+    ,
+    gs [mem_every_thm, mem_filter_thm, oEL_THM]
+  Cases_on ‘bir_get_stmt p s.bst_pc’ >> (simp [])
+  >| [
+    (* read *)
+    rw [bir_state_t_component_equality, eval_clstep_read_def, mem_read_view_def, mem_readable_def, mem_filter_def] >|
+QED
+
+
+Theorem LIST_TO_SET_MEM:
+  ∀x l.
+  set l x = MEM x l
+Proof
+  Induct_on ‘l’ >> (simp [])
+QED
+
+Theorem eval_clstep_correctness:
+  ∀p cid s M s'.
+  set (eval_clstep cid p s M) s' = ∃l. clstep p cid s M l s'
+Proof
+  rpt strip_tac >> EQ_TAC >>
+  (simp [LIST_TO_SET_MEM, eval_clstep_completeness, eval_clstep_soundness])
+QED
+
+val _ = export_theory();
